Fresh.v
@@ -1,7 +1,7 @@
 Require Import CSet Le Arith.Compare_dec.
 
 Require Import Plus Util Map.
-Require Import Env EnvTy IL.
+Require Import Env EnvTy IL InjectiveMapping.
 
 Set Implicit Arguments.
 
@@ -22,13 +22,6 @@ Section PolyIter.
     end.
 
 End PolyIter.
-
-Definition least_fresh (lv:set var) : var :=
-  let mx := fold max lv 0 in
-  let vx := iter (cardinal lv + 1)
-                 mx
-                 (fun n x => if [n ∈ lv] then x else n) in
-  vx.
 
 Definition fresh (s : set var) : var :=
   S(fold max s 0).
@@ -58,6 +51,33 @@ Proof.
   pose proof (fresh_spec' H). omega.
 Qed.
 
+Definition least_fresh (lv:set var) : var :=
+  let mx := S (fold max lv 0) in
+  let vx := iter (1 + cardinal lv)
+                 mx
+                 (fun n x => if [n ∈ lv] then x else n) in
+  vx.
+
+Lemma least_fresh_spec' G k mx
+: mx ∉ G
+  -> iter k mx (fun n x => if [n ∈ G] then x else n) ∉ G.
+Proof.
+  intros; intro.
+  general induction k; simpl in *.
+  - cset_tac; intuition.
+  - eapply IHk; try eapply H0; eauto.
+    destruct if; eauto.
+Qed.
+
+Lemma least_fresh_spec G
+: least_fresh G ∉ G.
+Proof.
+  eapply least_fresh_spec'.
+  intro.
+  pose proof (fresh_spec' H). omega.
+Qed.
+
+
 Definition fresh_stable (lv:set var) (x:var) : var :=
   if [x ∉ lv] then x else
     fresh lv.
@@ -68,88 +88,53 @@ Proof.
   unfold fresh_stable. destruct if; eauto using fresh_spec.
 Qed.
 
+Section FreshList.
 
-Fixpoint fresh_list (G:set var) (n:nat) : list var :=
-  match n with
-    | 0 => nil
-    | S n => let x := fresh G in x::fresh_list (G ∪ {{x}}) n
-  end.
+  Variable fresh : set var -> var.
 
-Definition fresh_set (G:set var) (n:nat) : set var :=
-  of_list (fresh_list G n).
+  Fixpoint fresh_list (G:set var) (n:nat) : list var :=
+    match n with
+      | 0 => nil
+      | S n => let x := fresh G in x::fresh_list (G ∪ {{x}}) n
+    end.
 
-Lemma fresh_list_spec : forall (G:set var) n, (of_list (fresh_list G n)) ∩ G [=] ∅.
-Proof.
-  intros. general induction n; simpl; split; intros.
-  cset_tac; eauto. exfalso; cset_tac; eauto.
-  cset_tac; intuition.
-  rewrite <- H in H1. eapply fresh_spec; eauto.
-  specialize (IHn (G ∪ {{fresh G}})). intuition (cset_tac; eauto).
-  exfalso; cset_tac; eauto.
-Qed.
-
-Lemma fresh_list_length (G:set var) n
+  Lemma fresh_list_length (G:set var) n
   : length (fresh_list G n) = n.
-Proof.
-  general induction n; eauto. simpl. f_equal; eauto.
-Qed.
+  Proof.
+    general induction n; eauto. simpl. f_equal; eauto.
+  Qed.
 
-Lemma fresh_set_spec
-: forall (G:set var) n, (fresh_set G n) ∩ G [=] ∅.
-Proof.
-  unfold fresh_set. eapply fresh_list_spec.
-Qed.
+  Hypothesis fresh_spec : forall G, fresh G ∉ G.
 
-Lemma fresh_list_unique (G: set var) n
-  : unique (fresh_list G n).
-Proof.
-  general induction n; simpl; eauto.
-  split; eauto. intro.
-  eapply (not_in_empty (fresh G)).
-  eapply fresh_list_spec.
-  cset_tac. eapply InA_in; eauto.
-  cset_tac; eauto.
-Qed.
+  Definition fresh_set (G:set var) (n:nat) : set var :=
+    of_list (fresh_list G n).
 
-Fixpoint fresh_stable_list (G:set var) (Z:list var) : list var :=
-  match Z with
-    | nil => nil
-    | x::Z' => let x' := fresh_stable (G ∪ of_list Z') x in x'::fresh_stable_list (G ∪ {{x'}}) Z'
-  end.
+  Lemma fresh_list_spec : forall (G:set var) n, (of_list (fresh_list G n)) ∩ G [=] ∅.
+  Proof.
+    intros. general induction n; simpl; split; intros; try now (cset_tac; intuition).
+    - cset_tac; intuition.
+      + invc H; eauto.
+      + specialize (H0 (G ∪ {{fresh G}})).
+        intuition (cset_tac; eauto).
+  Qed.
 
-Lemma fresh_stable_list_length (G:set var) Z
-  : length (fresh_stable_list G Z) = length Z.
-Proof.
-  general induction Z; eauto. simpl. f_equal; eauto.
-Qed.
+  Lemma fresh_set_spec
+  : forall (G:set var) n, (fresh_set G n) ∩ G [=] ∅.
+  Proof.
+    unfold fresh_set. eapply fresh_list_spec.
+  Qed.
 
-Lemma fresh_stable_list_spec
-: forall (G:set var) Z, (of_list (fresh_stable_list G Z)) ∩ G [=] ∅.
-Proof.
-  intros. general induction Z; simpl; split; intros.
-  - cset_tac; eauto.
-  - exfalso; cset_tac; eauto.
-  - cset_tac; intuition.
-    + hnf in H; subst.
-      assert (fresh_stable (G ∪ of_list Z) a ∈ G ∪ of_list Z).
-      cset_tac; intuition.
-      eapply fresh_stable_spec; eauto.
-    + eapply (not_in_empty a0). rewrite <- IHZ.
-      intuition (cset_tac; eauto).
-      intuition (cset_tac; eauto).
-  - exfalso; cset_tac; auto.
-Qed.
-
-Lemma fresh_stable_list_unique (G: set var) n
-  : unique (fresh_stable_list G n).
-Proof.
-  general induction n; simpl; eauto.
-  split; eauto. intro.
-  eapply (not_in_empty (fresh_stable (G ∪ of_list n) a)).
-  eapply fresh_stable_list_spec.
-  cset_tac. eapply InA_in; eauto.
-  cset_tac; eauto.
-Qed.
+  Lemma fresh_list_unique (G: set var) n
+    : unique (fresh_list G n).
+  Proof.
+    general induction n; simpl; eauto.
+    split; eauto. intro.
+    eapply (not_in_empty (fresh G)).
+    eapply fresh_list_spec.
+    cset_tac. eapply InA_in; eauto.
+    cset_tac; eauto.
+  Qed.
+End FreshList.
 
 Definition notincl {X} `{OrderedType X} (s t: set X) := forall x, x ∈ s -> x ∉ t.
 
@@ -186,14 +171,91 @@ Qed.
 
 Lemma inverse_on_update_fresh_list (D:set var) (Z:list var) (ϱ ϱ' : var -> var)
  : inverse_on (D \ of_list Z) ϱ ϱ'
-  -> inverse_on D (update_with_list Z (fresh_list (lookup_set ϱ (D \ of_list Z)) (length Z)) ϱ)
-                 (update_with_list (fresh_list (lookup_set ϱ (D \ of_list Z)) (length Z)) Z ϱ').
+  -> inverse_on D (update_with_list Z (fresh_list fresh (lookup_set ϱ (D \ of_list Z)) (length Z)) ϱ)
+                 (update_with_list (fresh_list fresh (lookup_set ϱ (D \ of_list Z)) (length Z)) Z ϱ').
 Proof.
   intros. eapply inverse_on_update_fresh; eauto.
-  eapply fresh_list_unique.
+  eapply fresh_list_unique, fresh_spec.
   rewrite fresh_list_length; eauto.
   hnf; intros. intro. eapply (not_in_empty x).
-  eapply fresh_list_spec. cset_tac; eauto.
+  eapply fresh_list_spec; eauto using fresh_spec. cset_tac; eauto.
+Qed.
+
+Hint Extern 20 (Subset (?a \ _) ?a) => eapply minus_incl.
+Hint Extern 20 (Subset (?a \ _) ?a') => (is_evar a ; fail 1)
+                                        || (has_evar a ; fail 1)
+                                        || (is_evar a' ; fail 1)
+                                        || (has_evar a'; fail 1)
+                                        || eapply minus_incl.
+Hint Extern 20 => match goal with
+                   | [ H: ?a /\ ?b |- ?b ] => eapply H
+                   | [ H: ?a /\ ?b |- ?a ] => eapply H
+                 end.
+
+Section MapUpdate.
+  Open Scope fmap_scope.
+  Variable X : Type.
+  Context `{OrderedType X}.
+  Variable Y : Type.
+
+  Lemma update_unique_commute `{OrderedType Y} (XL:list X) (VL:list Y) E D x y
+  : length XL = length VL
+    -> unique (x::XL)
+    -> agree_on _eq D (E [x <- y] [XL <-- VL]) (E [XL <-- VL] [x <- y]).
+  Proof.
+    intros. eapply length_length_eq in H1.
+    general induction H1; simpl. reflexivity.
+    hnf; intros. lud. hnf in H2; simpl in *.
+    dcr. exfalso. eapply H8. econstructor. eapply H5.
+    exploit (IHlength_eq H _ E {x1} x0 y0). simpl in *; intuition.
+    hnf; intros. eapply H9. econstructor 2; eauto.
+    exploit X0. cset_tac; reflexivity. rewrite X1. lud.
+    exploit (IHlength_eq H _ E {x1} x0 y0). simpl in *; intuition.
+    hnf; intros. eapply H8. econstructor 2; eauto.
+    exploit X0. cset_tac; reflexivity. rewrite X1. lud.
+  Qed.
+
+  Lemma injective_on_agree `{OrderedType Y} D (ϱ ϱ': X -> Y)
+  : injective_on D ϱ
+    -> agree_on _eq D ϱ ϱ'
+    -> injective_on D ϱ'.
+  Proof.
+    intros. hnf; intros. eapply H1; eauto.
+    exploit H2; eauto. rewrite X0.
+    exploit H2; try eapply H3. rewrite X1. eauto.
+  Qed.
+
+End MapUpdate.
+
+Lemma injective_on_fresh_list X `{OrderedType X} Y `{OrderedType Y} XL YL (ϱ: X -> Y) `{Proper _ (_eq ==> _eq) ϱ} lv
+: injective_on lv ϱ
+  -> length XL = length YL
+  -> (of_list YL) ∩ (lookup_set ϱ lv) [=] ∅
+  -> unique XL
+  -> unique YL
+  -> injective_on (lv ∪ of_list XL) (ϱ [XL <-- YL]).
+Proof.
+  intros. eapply length_length_eq in H3.
+  general induction H3; simpl in * |- * ; eauto.
+  - eapply injective_on_incl; eauto. cset_tac; intuition.
+  - eapply injective_on_agree.
+    assert (lv ∪ { x; of_list XL} [=] {{x}} ∪ lv ∪ of_list XL) by (cset_tac; intuition; eauto).
+    rewrite H7. eapply IHlength_eq; auto.
+    Focus 2.
+    eapply injective_on_fresh. instantiate (1:=ϱ); eauto.
+    eapply injective_on_incl; eauto. instantiate (1:=y).
+    intro. eapply lookup_set_spec in H8. dcr.
+    eapply (not_in_empty (ϱ x0)). rewrite <- H4. cset_tac; intuition.
+    eapply lookup_set_spec; eauto. eapply H1.
+    hnf; intros. lud; eauto; try now exfalso; eauto.
+    dcr. cset_tac; intuition.
+    eapply lookup_set_spec in H12; dcr. lud.
+    eapply H8. rewrite <- H14; eauto. eapply InA_in; eauto.
+    cset_tac; intuition.
+    eapply H4. split. right; eauto.
+    eapply lookup_set_spec. eauto. eexists; eauto.
+    hnf; intros. lud; eauto; try now exfalso; eauto.
+    eapply update_unique_commute; eauto using length_eq_length.
 Qed.
 
 
